thys/Pattern_Completeness/Pattern_Completeness_Set.thy
@@ -1529,112 +1529,72 @@ next
 qed 
 end
 
-context pattern_completeness_context begin
-
-text \<open>Conditions when all patterns are reduced to variables,
-   all var-conflicts for finite sorts are between variables (no function symbols),
-   and all var-conflicts give rise to a var-conflict of an infinite sort that occurs at root,
-   moreover, no obvious clashes are present.
-\<close>
-definition weak_finite_var_form_mp :: "('f,'v,'s)match_problem_set \<Rightarrow> bool" where
-  "weak_finite_var_form_mp mp = ((\<forall> (t,l) \<in> mp. \<exists> y. l = Var y)
-     \<and> (\<forall> f ts y. (Fun f ts, Var y) \<in> mp \<longrightarrow>  
-          (\<exists> x. (Var x, Var y) \<in> mp \<and> inf_sort (snd x))
-        \<and> (\<forall> t. (t, Var y) \<in> mp \<longrightarrow> root t \<in> {None, Some (f,length ts)})))"
-
 text \<open>Represent a variable-form as a set of maps.\<close>
 
-definition "mp_var_form f = {(Var y, Var x) | x y. y \<in> f x}"
+definition "match_of_var_form f = {(Var y, Var x) | x y. y \<in> f x}"
 
-definition "pp_var_form ff = mp_var_form ` ff"
+definition "pat_of_var_form ff = match_of_var_form ` ff"
 
-definition "var_form_of_mp mp x = {y. (Var y, Var x) \<in> mp}"
+definition "var_form_of_match mp x = {y. (Var y, Var x) \<in> mp}"
 
-definition "var_form_of_pp pp = var_form_of_mp ` pp"
+definition "var_form_of_pat pp = var_form_of_match ` pp"
 
-definition "vars_var_form_pp ff = (\<Union>f \<in> ff. \<Union>(range f))"
+definition "tvars_var_form_pat ff = (\<Union>f \<in> ff. \<Union>(range f))"
 
-definition var_form_mp where
-  "var_form_mp mp \<longleftrightarrow> mp \<subseteq> range (map_prod Var Var)"
+definition var_form_match where
+  "var_form_match mp \<longleftrightarrow> mp \<subseteq> range (map_prod Var Var)"
 
-definition "var_form_pp pp \<equiv> \<forall>mp \<in> pp. var_form_mp mp"
+definition "var_form_pat pp \<equiv> \<forall>mp \<in> pp. var_form_match mp"
 
-definition finite_var_form_mp :: "('f,'v,'s)match_problem_set \<Rightarrow> bool" where
-  "finite_var_form_mp mp \<longleftrightarrow> var_form_mp mp \<and>
-  (\<forall>l x y. (Var x, l) \<in> mp \<longrightarrow> (Var y, l) \<in> mp \<longrightarrow> snd x = snd y) \<and>
-  (\<forall>l x. (Var x, l) \<in> mp \<longrightarrow> \<not> inf_sort (snd x))"
-
-lemma finite_var_form_mpD:
-  assumes "finite_var_form_mp mp" and "(t,l) \<in> mp"
-  shows "\<exists>x \<iota> y. t = Var (x,\<iota>) \<and> l = Var y \<and> \<not> inf_sort \<iota> \<and>
-    (\<forall>z. (Var z, Var y) \<in> mp \<longrightarrow> snd z = \<iota>)"
-  using assms by (auto simp: finite_var_form_mp_def var_form_mp_def)
-
-definition weak_finite_var_form_pp :: "('f,'v,'s)pat_problem_set \<Rightarrow> bool" where
-  "weak_finite_var_form_pp p = (\<forall> mp \<in> p. weak_finite_var_form_mp mp)"
-
-definition finite_var_form_pp :: "('f,'v,'s)pat_problem_set \<Rightarrow> bool" where
-  "finite_var_form_pp p = (\<forall> mp \<in> p. finite_var_form_mp mp)"
-
-lemma finite_var_form_ppD:
-  assumes "finite_var_form_pp pp" "mp \<in> pp" "(t,l) \<in> mp"
-  shows "\<exists>x \<iota> y. t = Var (x,\<iota>) \<and> l = Var y \<and> \<not> inf_sort \<iota> \<and>
-    (\<forall>z. (Var z, Var y) \<in> mp \<longrightarrow> snd z = \<iota>)"
-  using assms[unfolded finite_var_form_pp_def] finite_var_form_mpD by metis
-
-lemma finite_var_form_imp_var_form_pp:
-  "finite_var_form_pp pp \<Longrightarrow> var_form_pp pp"
-  by (auto simp: finite_var_form_pp_def var_form_pp_def finite_var_form_mp_def)
-
-lemma mp_var_form_of_mp:
-  assumes "var_form_mp mp"
-  shows "mp_var_form (var_form_of_mp mp) = mp"
+lemma match_of_var_form_of_match:
+  assumes "var_form_match mp"
+  shows "match_of_var_form (var_form_of_match mp) = mp"
   using assms
-  by (auto simp: var_form_mp_def mp_var_form_def var_form_of_mp_def)
+  by (auto simp: var_form_match_def match_of_var_form_def var_form_of_match_def)
 
-lemma pp_var_form_pat:
-  assumes "var_form_pp pp"
-  shows "pp_var_form (var_form_of_pp pp) = pp"
-  using assms mp_var_form_of_mp
-  by (auto simp: var_form_pp_def var_form_of_pp_def pp_var_form_def)
+lemma pat_of_var_form_pat:
+  assumes "var_form_pat pp"
+  shows "pat_of_var_form (var_form_of_pat pp) = pp"
+  using assms match_of_var_form_of_match
+  by (auto simp: var_form_pat_def var_form_of_pat_def pat_of_var_form_def)
 
-lemma tvars_pat_var_form: "tvars_pat (pp_var_form ff) = vars_var_form_pp ff"
-  by (fastforce simp: vars_var_form_pp_def tvars_pat_def tvars_mp_def pp_var_form_def mp_var_form_def
+lemma tvars_pat_var_form: "tvars_pat (pat_of_var_form ff) = tvars_var_form_pat ff"
+  by (fastforce simp: tvars_var_form_pat_def tvars_pat_def tvars_mp_def pat_of_var_form_def match_of_var_form_def
       split: prod.splits)
 
-lemma vars_var_form_pp:
-  assumes "var_form_pp pp"
-  shows "vars_var_form_pp (var_form_of_pp pp) = tvars_pat pp"
-  apply (subst(2) pp_var_form_pat[OF assms,symmetric])
+lemma tvars_var_form_pat:
+  assumes "var_form_pat pp"
+  shows "tvars_var_form_pat (var_form_of_pat pp) = tvars_pat pp"
+  apply (subst(2) pat_of_var_form_pat[OF assms,symmetric])
   by (simp add: tvars_pat_var_form)
 
 lemma pat_complete_var_form:
-  "pat_complete C (pp_var_form ff) \<longleftrightarrow>
-  (\<forall>\<sigma> :\<^sub>s \<V> |` vars_var_form_pp ff \<rightarrow> \<T>(C). \<exists>f \<in> ff. \<exists>\<mu>. \<forall>x. \<forall>y \<in> f x. \<sigma> y = \<mu> x)"
+  "pat_complete C (pat_of_var_form ff) \<longleftrightarrow>
+  (\<forall>\<sigma> :\<^sub>s \<V> |` tvars_var_form_pat ff \<rightarrow> \<T>(C). \<exists>f \<in> ff. \<exists>\<mu>. \<forall>x. \<forall>y \<in> f x. \<sigma> y = \<mu> x)"
 proof-
-  define V where "V = \<V> |` vars_var_form_pp ff"
+  define V where "V = \<V> |` tvars_var_form_pat ff"
   have boo: "\<V> |` tvars_pat {{(Var (a, b), Var xa) | xa a b. (a, b) \<in> x xa} |. x \<in> ff} = V"
     apply (unfold V_def)
     apply (subst tvars_pat_var_form[of ff, symmetric])
-    by (auto simp: V_def pp_var_form_def mp_var_form_def)
+    by (auto simp: V_def pat_of_var_form_def match_of_var_form_def)
   show ?thesis
     apply (fold V_def)
-    apply (auto simp: pat_complete_def match_complete_wrt_def pp_var_form_def
-      mp_var_form_def imp_conjL imp_ex boo)
+    apply (auto simp: pat_complete_def match_complete_wrt_def pat_of_var_form_def
+      match_of_var_form_def imp_conjL imp_ex boo)
     apply (metis old.prod.exhaust)
     by metis
 qed
 
 lemma pat_complete_var_form_set:
-  "pat_complete C (pp_var_form ff) \<longleftrightarrow>
-  (\<forall>\<sigma> :\<^sub>s \<V> |` vars_var_form_pp ff \<rightarrow> \<T>(C). \<exists>f \<in> ff. \<exists>\<mu>. \<forall>x. \<sigma> ` f x \<subseteq> {\<mu> x})"
+  "pat_complete C (pat_of_var_form ff) \<longleftrightarrow>
+  (\<forall>\<sigma> :\<^sub>s \<V> |` tvars_var_form_pat ff \<rightarrow> \<T>(C). \<exists>f \<in> ff. \<exists>\<mu>. \<forall>x. \<sigma> ` f x \<subseteq> {\<mu> x})"
   by (auto simp: pat_complete_var_form image_subset_iff)
 
 lemma pat_complete_var_form_Uniq:
-  "pat_complete C (pp_var_form ff) \<longleftrightarrow>
-  (\<forall>\<sigma> :\<^sub>s \<V> |` vars_var_form_pp ff \<rightarrow> \<T>(C). \<exists>f \<in> ff. \<forall>x. UNIQ (\<sigma> ` f x))"
+  "pat_complete C (pat_of_var_form ff) \<longleftrightarrow>
+  (\<forall>\<sigma> :\<^sub>s \<V> |` tvars_var_form_pat ff \<rightarrow> \<T>(C). \<exists>f \<in> ff. \<forall>x. UNIQ (\<sigma> ` f x))"
 proof-
-  { fix \<sigma> f assume \<sigma>: "\<sigma> :\<^sub>s \<V> |` vars_var_form_pp ff \<rightarrow> \<T>(C)" and f: "f \<in> ff"
+  { fix \<sigma> f assume \<sigma>: "\<sigma> :\<^sub>s \<V> |` tvars_var_form_pat ff \<rightarrow> \<T>(C)" and f: "f \<in> ff"
     have "(\<exists>\<mu>. \<forall>x. \<sigma> ` f x \<subseteq> {\<mu> x}) \<longleftrightarrow> (\<forall>x. \<exists>\<^sub>\<le>\<^sub>1 y. y \<in> \<sigma> ` f x)"
     proof (safe)
       fix \<mu> x
@@ -1652,38 +1612,33 @@ proof-
   then show ?thesis by (simp add: pat_complete_var_form_set)
 qed
 
-lemma ex_var_form_pp: "(\<exists>f\<in>var_form_of_pp pp. P f) \<longleftrightarrow> (\<exists>mp \<in> pp. P (var_form_of_mp mp))"
-  by (auto simp: var_form_of_pp_def)
-
-end
-
-context pattern_completeness_context_with_assms begin
+lemma ex_var_form_pat: "(\<exists>f\<in>var_form_of_pat pp. P f) \<longleftrightarrow> (\<exists>mp \<in> pp. P (var_form_of_match mp))"
+  by (auto simp: var_form_of_pat_def)
 
 lemma pat_complete_var_form_nat:
-  assumes finS: "\<forall>(x,\<iota>) \<in> vars_var_form_pp ff. \<iota> \<in> S \<and> finite_sort C \<iota>"
+  assumes fin: "\<forall>(x,\<iota>) \<in> tvars_var_form_pat ff. finite_sort C \<iota>"
     and uniq: "\<forall>f \<in> ff. \<forall>x::'v. UNIQ (snd ` f x)"
-  shows "pat_complete C (pp_var_form ff) \<longleftrightarrow>
-  (\<forall>\<alpha>. (\<forall>(x,\<iota>) \<in> vars_var_form_pp ff. \<alpha> (x,\<iota>) < card_of_sort C \<iota>) \<longrightarrow>
+  shows "pat_complete C (pat_of_var_form ff) \<longleftrightarrow>
+  (\<forall>\<alpha>. (\<forall>(x,\<iota>) \<in> tvars_var_form_pat ff. \<alpha> (x,\<iota>) < card_of_sort C \<iota>) \<longrightarrow>
   (\<exists>f \<in> ff. \<forall>x. UNIQ (\<alpha> ` f x)))"
   (is "?l \<longleftrightarrow> (\<forall>\<alpha>. ?s \<alpha> \<longrightarrow> ?r \<alpha>)")
 proof safe
-  note finS[unfolded Ball_Pair_conv, rule_format]
-  note fin = this[THEN conjunct2] and S = this[THEN conjunct1]
+  note fin = fin[unfolded Ball_Pair_conv, rule_format]
   { fix \<alpha>
     assume l: ?l and a: "?s \<alpha>"
-    define \<sigma> :: "_ \<Rightarrow> ('f,unit) term" where
+    define \<sigma> :: "_ \<Rightarrow> (_,unit) term" where
       "\<sigma> \<equiv> \<lambda>(x,\<iota>). term_of_index C \<iota> (\<alpha> (x,\<iota>))"
-    have "\<sigma> (x,\<iota>) : \<iota> in \<T>(C)" if x: "(x,\<iota>) \<in> vars_var_form_pp ff" for x \<iota>
+    have "\<sigma> (x,\<iota>) : \<iota> in \<T>(C)" if x: "(x,\<iota>) \<in> tvars_var_form_pat ff" for x \<iota>
       using term_of_index_bij[OF fin, OF x]
         a[unfolded Ball_Pair_conv, rule_format, OF x]
       by (auto simp: bij_betw_def \<sigma>_def)
-    then have "\<sigma> :\<^sub>s \<V> |` vars_var_form_pp ff \<rightarrow> \<T>(C)"
+    then have "\<sigma> :\<^sub>s \<V> |` tvars_var_form_pat ff \<rightarrow> \<T>(C)"
       by (auto intro!: sorted_mapI simp: hastype_restrict)
     from l[unfolded pat_complete_var_form_Uniq, rule_format, OF this]
     obtain f where f: "f \<in> ff" and u: "\<And>x. UNIQ (\<sigma> ` f x)" by auto
     have id: "y \<in> f x \<Longrightarrow> index_of_term C (\<sigma> y) = \<alpha> y" for y x
       using assms a f
-      by (auto simp: \<sigma>_def index_of_term_of_index vars_var_form_pp_def split: prod.splits)
+      by (auto simp: \<sigma>_def index_of_term_of_index tvars_var_form_pat_def split: prod.splits)
     then have "\<alpha> ` f x = index_of_term C ` \<sigma> ` f x" for x
       by (auto simp: image_def)
     then have "UNIQ (\<alpha> ` f x)" for x by (simp add: image_Uniq[OF u])
@@ -1694,12 +1649,12 @@ proof safe
       unfolding pat_complete_var_form_Uniq
     proof safe
       fix \<sigma>
-      assume \<sigma>: "\<sigma> :\<^sub>s \<V> |` vars_var_form_pp ff \<rightarrow> \<T>(C)"
+      assume \<sigma>: "\<sigma> :\<^sub>s \<V> |` tvars_var_form_pat ff \<rightarrow> \<T>(C)"
       from sorted_mapD[OF this]
-      have ty: "(x,\<iota>) \<in> vars_var_form_pp ff \<Longrightarrow> \<sigma> (x,\<iota>) : \<iota> in \<T>(C)"
-        for x \<iota> using S by (auto simp: hastype_restrict)
+      have ty: "(x,\<iota>) \<in> tvars_var_form_pat ff \<Longrightarrow> \<sigma> (x,\<iota>) : \<iota> in \<T>(C)"
+        for x \<iota> by (auto simp: hastype_restrict)
       define \<alpha> where "\<alpha> \<equiv> index_of_term C \<circ> \<sigma>"
-      have "\<alpha> (x,\<iota>) < card_of_sort C \<iota>" if x: "(x,\<iota>) \<in> vars_var_form_pp ff"
+      have "\<alpha> (x,\<iota>) < card_of_sort C \<iota>" if x: "(x,\<iota>) \<in> tvars_var_form_pat ff"
         for x \<iota> using index_of_term_bij[OF fin[OF x]] ty[OF x]
         by (auto simp: \<alpha>_def bij_betw_def)
       then have "\<exists>f\<in>ff. \<forall>x. UNIQ (\<alpha> ` f x)" by (auto intro!: r[rule_format])
@@ -1712,9 +1667,9 @@ proof safe
         then obtain \<iota> where sub: "snd ` f x \<subseteq> {\<iota>}" by auto
         { fix y \<kappa> assume yk: "(y,\<kappa>) \<in> f x"
           with sub have [simp]: "\<kappa> = \<iota>" by auto 
-          from yk f have y: "(y,\<iota>) \<in> vars_var_form_pp ff"
-            by (auto simp: vars_var_form_pp_def)
-          from S[OF y] y fin[OF y]
+          from yk f have y: "(y,\<iota>) \<in> tvars_var_form_pat ff"
+            by (auto simp: tvars_var_form_pat_def)
+          from y fin[OF y]
           have "term_of_index C \<iota> (\<alpha> (y,\<kappa>)) = \<sigma> (y,\<kappa>)"
             by (auto simp: \<alpha>_def hastype_restrict
                 intro!: term_of_index_of_term sorted_mapD[OF \<sigma>])
@@ -1730,61 +1685,93 @@ proof safe
   }
 qed
 
-context
-  fixes pp
-  assumes fvf: "finite_var_form_pp pp"
-    and wf: "wf_pat pp"
-begin
+text \<open>Conditions when all patterns are reduced to variables,
+   all var-conflicts for finite sorts are between variables (no function symbols),
+   and all var-conflicts give rise to a var-conflict of an infinite sort that occurs at root,
+   moreover, no obvious clashes are present.
+\<close>
 
-private lemma vf: "var_form_pp pp"
-  using finite_var_form_imp_var_form_pp[OF fvf].
+definition finite_var_form_match :: "('f,'s) ssig \<Rightarrow> ('f,'v,'s)match_problem_set \<Rightarrow> bool" where
+  "finite_var_form_match C mp \<longleftrightarrow> var_form_match mp \<and>
+  (\<forall>l x y. (Var x, l) \<in> mp \<longrightarrow> (Var y, l) \<in> mp \<longrightarrow> snd x = snd y) \<and>
+  (\<forall>l x. (Var x, l) \<in> mp \<longrightarrow> finite_sort C (snd x))"
 
-lemma tvars_pat_S: assumes y: "(y,\<iota>) \<in> tvars_pat pp" shows "\<iota> \<in> S"
-  using wf y by (auto simp: wf_pat_def wf_match_iff tvars_pat_def)
+lemma finite_var_form_matchD:
+  assumes "finite_var_form_match C mp" and "(t,l) \<in> mp"
+  shows "\<exists>x \<iota> y. t = Var (x,\<iota>) \<and> l = Var y \<and> finite_sort C \<iota> \<and>
+    (\<forall>z. (Var z, Var y) \<in> mp \<longrightarrow> snd z = \<iota>)"
+  using assms by (auto simp: finite_var_form_match_def var_form_match_def)
 
-lemma tvars_pat_finite: assumes y: "(y,\<iota>) \<in> tvars_pat pp" shows "finite_sort C \<iota>"
-proof-
-  from y obtain mp t l where mp: "mp \<in> pp" and tl:"(t,l) \<in> mp" and yt: "(y, \<iota>) \<in> vars t"
-    by (auto simp: tvars_pat_def tvars_mp_def)
-  from finite_var_form_ppD[OF fvf mp tl] yt have "\<not> inf_sort \<iota>" by auto
-  with tvars_pat_S[OF y] inf_sort
-  show ?thesis by auto
-qed
+definition finite_var_form_pat :: "('f,'s) ssig \<Rightarrow> ('f,'v,'s)pat_problem_set \<Rightarrow> bool" where
+  "finite_var_form_pat C p = (\<forall> mp \<in> p. finite_var_form_match C mp)"
 
-lemma UNIQ_sort: assumes f: "f \<in> var_form_of_pp pp" shows "UNIQ (snd ` f x)"
+lemma finite_var_form_patD:
+  assumes "finite_var_form_pat C pp" "mp \<in> pp" "(t,l) \<in> mp"
+  shows "\<exists>x \<iota> y. t = Var (x,\<iota>) \<and> l = Var y \<and> finite_sort C \<iota> \<and>
+    (\<forall>z. (Var z, Var y) \<in> mp \<longrightarrow> snd z = \<iota>)"
+  using assms[unfolded finite_var_form_pat_def] finite_var_form_matchD by metis
+
+lemma finite_var_form_imp_of_var_form_pat:
+  "finite_var_form_pat C pp \<Longrightarrow> var_form_pat pp"
+  by (auto simp: finite_var_form_pat_def var_form_pat_def finite_var_form_match_def)
+
+context pattern_completeness_context begin
+
+definition weak_finite_var_form_match :: "('f,'v,'s)match_problem_set \<Rightarrow> bool" where
+  "weak_finite_var_form_match mp = ((\<forall> (t,l) \<in> mp. \<exists> y. l = Var y)
+     \<and> (\<forall> f ts y. (Fun f ts, Var y) \<in> mp \<longrightarrow>  
+          (\<exists> x. (Var x, Var y) \<in> mp \<and> inf_sort (snd x))
+        \<and> (\<forall> t. (t, Var y) \<in> mp \<longrightarrow> root t \<in> {None, Some (f,length ts)})))"
+
+definition weak_finite_var_form_pat :: "('f,'v,'s)pat_problem_set \<Rightarrow> bool" where
+  "weak_finite_var_form_pat p = (\<forall> mp \<in> p. weak_finite_var_form_match mp)"
+
+end
+
+lemma finite_var_form_pat_UNIQ_sort:
+  assumes fvf: "finite_var_form_pat C pp"
+    and f: "f \<in> var_form_of_pat pp"
+  shows "UNIQ (snd ` f x)"
 proof (intro Uniq_I, clarsimp)
-  from f obtain mp where mp: "mp \<in> pp" and f: "f = var_form_of_mp mp"
-    by (auto simp: var_form_of_pp_def)
+  from f obtain mp where mp: "mp \<in> pp" and f: "f = var_form_of_match mp"
+    by (auto simp: var_form_of_pat_def)
   fix y \<iota> z \<kappa> assume "(y,\<iota>) \<in> f x" "(z,\<kappa>) \<in> f x"
   with f have y: "(Var (y,\<iota>), Var x) \<in> mp" and z: "(Var (z,\<kappa>), Var x) \<in> mp"
-    by (auto simp: var_form_of_mp_def)
-  from finite_var_form_ppD[OF fvf mp y] z
+    by (auto simp: var_form_of_match_def)
+  from finite_var_form_patD[OF fvf mp y] z
   show "\<iota> = \<kappa>" by auto
 qed
 
-lemma finite_var_form_pp_pat_complete: "pat_complete C pp \<longleftrightarrow>
-  (\<forall>\<alpha>. (\<forall>(y,\<iota>) \<in> tvars_pat pp. \<alpha> (y,\<iota>) < card_of_sort C \<iota>) \<longrightarrow>
+lemma finite_var_form_pat_pat_complete:
+  assumes fvf: "finite_var_form_pat C pp"
+  shows "pat_complete C pp \<longleftrightarrow>
+    (\<forall>\<alpha>. (\<forall>(y,\<iota>) \<in> tvars_pat pp. \<alpha> (y,\<iota>) < card_of_sort C \<iota>) \<longrightarrow>
     (\<exists>mp \<in> pp. \<forall>x. UNIQ {\<alpha> y |y. (Var y, Var x) \<in> mp}))"
 proof-
-  note pat_complete_var_form_nat[of "var_form_of_pp pp"]
-  note this[unfolded pp_var_form_pat[OF vf]]
-  note * = this[unfolded vars_var_form_pp[OF vf]]
+  note vf = finite_var_form_imp_of_var_form_pat[OF fvf]
+  note pat_complete_var_form_nat[of "var_form_of_pat pp" C]
+  note this[unfolded tvars_var_form_pat[OF vf]]
+  note * = this[unfolded pat_of_var_form_pat[OF vf]]
   show ?thesis
     apply (subst *)
-    subgoal using tvars_pat_finite tvars_pat_S by force
-    subgoal using UNIQ_sort by force
+    subgoal
+    proof
+      fix y \<iota>
+      assume y: "(y,\<iota>) \<in> tvars_pat pp"
+      from y obtain mp t l where mp: "mp \<in> pp" and tl:"(t,l) \<in> mp" and yt: "(y, \<iota>) \<in> vars t"
+        by (auto simp: tvars_pat_def tvars_mp_def)
+      from finite_var_form_patD[OF fvf mp tl] yt
+      show "finite_sort C \<iota>" by auto
+    qed
+    subgoal using finite_var_form_pat_UNIQ_sort[OF fvf] by force
     subgoal 
       apply (rule all_cong)
-      apply (unfold ex_var_form_pp)
+      apply (unfold ex_var_form_pat)
       apply (rule bex_cong[OF refl])
       apply (rule all_cong1)
       apply (rule arg_cong[of _ _ UNIQ])
-      by (auto simp: var_form_of_mp_def)
+      by (auto simp: var_form_of_match_def)
     done
 qed
-
-end
-
-end
 
 end
